WIP; jobs being done should have return values

helping/elim_stack/StackA.v
@@ -13,6 +13,43 @@ Global Instance subG_stackG `{!crisG Γ Σ α β τ _S _I} : subG stackΓ Γ →
 Proof. solve_inG. Defined.
 Hint Unfold subG_stackG stack_tokG stack_stateG : GRA_index.
 
+Class SLRed `{Σ : GRA, @GATIntp.t (domain Σ) α} {n} (f : GTerm.t n) (P : iProp Σ) := {
+  SLRed_eq : ⟦f⟧ ⊣⊢ P
+}.
+Lemma SLRed_red `{S : SLRed n f P} : ⟦f⟧ ⊣⊢ P.
+Proof. destruct S; ss. Qed.
+
+Section instances.
+  Context `{!subG (Γ : HRA) Σ, !SL.G Γ Σ α β τ}.
+
+  Global Instance SLRed_own `{!inG M Γ, n : nat} (m : M) γ :
+    SLRed (n:=n) (<own> γ m)%SAT (own γ m).
+  Proof. econs; SL_red; eauto. Qed.
+
+  Global Instance SLRed_pure {n} (P : Prop) :
+    SLRed (⌜P⌝ : GTerm.t n)%SAT (⌜P⌝)%I.
+  Proof. econs; SL_red; eauto. Qed.
+
+  Global Instance SLRed_ex {A n} `{!STτ.t τ}
+      (f : A → GTerm.t n) (g : A → iProp Σ) `{∀ a, SLRed (f a) (g a)} :
+    SLRed (∃ a : τ{A}, f a)%SAT (∃ a, g a)%I.
+  Proof.
+    econs; SL_red; iSplit; iIntros "[%b H]"; iExists b; try rewrite SLRed_red //.
+  Qed.
+
+  Global Instance SLRed_and {n} (f g : GTerm.t n) P Q `{!SLRed f P, !SLRed g Q} :
+    SLRed (f ∧ g)%SAT (P ∧ Q).
+  Proof. econs; rewrite SLRed.and ?SLRed_red //. Qed.
+
+  Global Instance SLRed_or {n} (f g : GTerm.t n) P Q `{!SLRed f P, !SLRed g Q} :
+    SLRed (f ∨ g)%SAT (P ∨ Q).
+  Proof. econs; rewrite SLRed.or ?SLRed_red //. Qed.
+
+  Global Instance SLRed_sep {n} (f g : GTerm.t n) P Q `{!SLRed f P, !SLRed g Q} :
+    SLRed (f ∗ g)%SAT (P ∗ Q).
+  Proof. econs; rewrite SLRed.sepconj ?SLRed_red //. Qed.
+End instances.
+
 Section definitions.
   Context `{!crisG Γ Σ α β τ _S _I, !concG, !memG, !stackG} (N : namespace).
 
@@ -29,29 +66,84 @@ Section definitions.
     iCombine "Hl1 Hl2" gives %[]%auth_frag_op_valid_1.
   Qed.
 
-  Definition stack_elem_to_val (stack_rep : option val) : val :=
+  (* Definition stack_elem_to_val (stack_rep : option val) : val :=
     match stack_rep with
     | None => Vint 0
     | Some l => l
-    end.
+    end. *)
 
-  Fixpoint list_inv (l : list val) (rep : option val) (n : nat) : GTerm.t n :=
+  Fixpoint syn_list_inv (l : list val) (rep : val) (n : nat) : GTerm.t n :=
     match l with
-    | nil => ⌜rep = None⌝
-    | v::l => ∃ (blk : τ{mblock}) (ofs : τ{ptrofs}) (rep' : τ{option val}),
-        ⌜rep = Some (Vptr (blk, ofs))⌝ ∗
-        (blk, ofs) ↦□ v ∗ (blk, ofs + 1)%Z ↦□ stack_elem_to_val rep' ∗ list_inv l rep' n
+    | nil => ⌜rep = Vint 0⌝
+    | v::l => ∃ (blk : τ{mblock}) (ofs : τ{ptrofs}) (rep' : τ{val}) (q0 q1 : τ{Qp}),
+        ⌜rep = Vptr (blk, ofs)⌝ ∗
+        (blk, ofs) ↦{q0} v ∗ (blk, ofs + 1)%Z ↦{q1} rep' ∗ syn_list_inv l rep' n
     end%SAT.
 
-  Definition is_offer (γs : gname) (offer_rep : option val) (n : nat) : GTerm.t n :=
+  Fixpoint list_inv (l : list val) (rep : val) (n : nat) : iProp Σ :=
+    match l with
+    | nil => ⌜rep = Vint 0⌝
+    | v::l => ∃ (blk : mblock) (ofs : ptrofs) (rep' : val) (q0 q1 : Qp),
+        ⌜rep = Vptr (blk, ofs)⌝ ∗
+        (blk, ofs) ↦{q0} v ∗ (blk, ofs + 1)%Z ↦{q1} rep' ∗ list_inv l rep' n
+    end%I.
+
+  Global Instance list_inv_SLRed l n rep : SLRed (syn_list_inv l rep n) (list_inv l rep n).
+  Proof. revert n rep; induction l; econs; rewrite SLRed_red //. Qed.
+  Local Hint Extern 0 (environments.envs_entails _ (list_inv (_::_) _)) => simpl : core.
+
+  Lemma list_inv_comparable l rep n :
+    list_inv l rep n -∗
+    list_inv l rep n ∗
+    (∃ q v, MemSpec.val_r rep q v) ∗
+    □ (∀ l' rep' n', list_inv l' rep' n' -∗ ∃ succ, ⌜MemSpec.compare_val rep' rep = Vint succ⌝).
+  Proof.
+    iIntros "L"; iAssert (⌜rep = Vint 0 ∨ ∃ b ofs, rep = Vptr (b, ofs)⌝)%I as "%".
+    { destruct l; ss; first iPoseProof "L" as "%"; eauto.
+      iDestruct "L" as "[% [% [% [% [% [-> ?]]]]]]"; iPureIntro; right; esplits; eauto.
+    }
+    iAssert (list_inv l rep n ∗ ∃ v q, MemSpec.val_r (rep) q v)%I
+      with "[L]" as "[L [% [% $]]]".
+    { destruct rep as [v'|v'|]; eauto. destruct v'; eauto.
+      destruct l; eauto.
+      { iPoseProof "L" as "%"; clarify. }
+      { iDestruct "L" as "[% [% [% [% [% [% [↦ R]]]]]]]". clarify; eauto.
+        iDestruct "↦" as "[↦1 ↦2]"; ss; iSplitR "↦1"; last iFrame.
+        iExists _, _, _, _, _; iSplit; first done. iFrame "↦2 R".
+      }
+    }
+
+    iFrame "L".
+    iIntros "!> % % % L"; destruct l'; ss.
+    { iPoseProof "L" as "->"; des; clarify; eauto. }
+    { iPoseProof "L" as "[% [% [% [% [% [-> ?]]]]]]"; des; clarify; iPureIntro; eauto; ss.
+      des_ifs; eauto.
+    }
+  Unshelve. all: try exact Vundef; try exact 1%Qp.
+  Qed.
+
+  Definition syn_is_offer (γs : gname) (offer_rep : option val) (n : nat) : GTerm.t n :=
     match offer_rep with
     | None => ⊤
     | Some l => ⊤
       (* ∃ Q γo, inv offerN (offer_inv st_loc γo (stack_push_au γs v Q) Q) *)
     end%SAT.
 
-  Local Instance is_offer_persistent γs offer_rep n : Persistent (⟦is_offer γs offer_rep n⟧).
-  Proof. rewrite /is_offer; destruct offer_rep as [?|]; SL_red; apply _. Qed.
+  Definition is_offer (γs : gname) (offer_rep : option val) (n : nat) : iProp Σ :=
+    match offer_rep with
+    | None => True
+    | Some l => True
+      (* ∃ Q γo, inv offerN (offer_inv st_loc γo (stack_push_au γs v Q) Q) *)
+    end%I.
+
+  Global Instance is_offer_SLRed γs offer_rep n :
+    SLRed (syn_is_offer γs offer_rep n) (is_offer γs offer_rep n).
+  Proof.
+    rewrite /syn_is_offer; destruct offer_rep; ss; econs; SL_red; eauto.
+  Qed.
+
+  Local Instance is_offer_persistent γs offer_rep n : Persistent (⟦syn_is_offer γs offer_rep n⟧).
+  Proof. rewrite SLRed_red. destruct offer_rep as [?|]; SL_red; apply _. Qed.
 
   Definition offer_to_val (offer_rep : option val) : val :=
     match offer_rep with
@@ -59,30 +151,35 @@ Section definitions.
     | Some l => l
     end.
 
-  Definition stack_inv (γs : gname) (stackb : mblock) (stackofs : ptrofs) (n : nat) : GTerm.t n :=
-    (∃ (stack_rep offer_rep : τ{option val}) (l : τ{list val}), <own> γs (● Excl' l) ∗
-       (stackb, stackofs) ↦ stack_elem_to_val stack_rep ∗ list_inv l stack_rep n ∗
-       (stackb, stackofs + 1)%Z ↦ offer_to_val offer_rep ∗ is_offer γs offer_rep n)%SAT.
+  Definition syn_stack_inv (γs : gname) (stackb : mblock) (stackofs : ptrofs) (n : nat) : GTerm.t n :=
+    (∃ (stack_rep : τ{val}) (offer_rep : τ{option val}) (l : τ{list val}), <own> γs (● Excl' l) ∗
+       (stackb, stackofs) ↦ stack_rep ∗ syn_list_inv l stack_rep n ∗
+       (stackb, stackofs + 1)%Z ↦ offer_to_val offer_rep ∗ syn_is_offer γs offer_rep n)%SAT.
+
+  Definition stack_inv (γs : gname) (stackb : mblock) (stackofs : ptrofs) (n : nat) : iProp Σ :=
+    (∃ (stack_rep : val) (offer_rep : option val) (l : list val), own γs (● Excl' l) ∗
+      (stackb, stackofs) ↦ stack_rep ∗ list_inv l stack_rep n ∗
+      (stackb, stackofs + 1)%Z ↦ offer_to_val offer_rep ∗ is_offer γs offer_rep n)%I.
+
+  Global Instance stack_inv_SLRed γs stackb stackofs n :
+    SLRed (syn_stack_inv γs stackb stackofs n) (stack_inv γs stackb stackofs n).
+  Proof. rewrite /syn_stack_inv /stack_inv; econs; rewrite SLRed_red //. Qed.
 
   Definition is_stack (γs : gname) (s : val) (n : nat) : iProp Σ :=
     (∃ (stackb : mblock) (stackofs : ptrofs),
-      ⌜s = Vptr (stackb, stackofs)⌝ ∗ inv n stackN (stack_inv γs stackb stackofs n))%I.
+      ⌜s = Vptr (stackb, stackofs)⌝ ∗ inv n stackN (syn_stack_inv γs stackb stackofs n))%I.
 
-  Definition new_stack_spec : fspecS :=
-    from_fspec
-      (fspec_winv (↑N)
-         (fspec_simple
-           (λ _ : (),
-            ((λ arg, ∃ (v : list val), ⌜arg = v↑⌝),
-             (λ ret, ∃ v γs, ⌜ret = v↑⌝ ∗ is_stack γs v 0 ∗ stack_content γs []))%I))).
+  Definition new_stack_spec : fspec :=
+    fspec_winv (↑N)
+      (fspec_simple (λ _ : (),
+        ((λ arg, ∃ (v : list val), ⌜arg = v↑⌝),
+         (λ ret, ∃ v γs, ⌜ret = v↑⌝ ∗ is_stack γs v 0 ∗ stack_content γs []))%I)).
 
-  Definition push_spec : fspecS :=
-    from_fspec
-      (fspec_winv (↑N)
-         (fspec_simple
-           (λ '((s, v, l, γs) : val * val * list (leibnizO val) * gname),
-            ((λ arg, ⌜arg = [s; v]↑⌝ ∗ is_stack γs s 0 ∗ stack_content γs l),
-             (λ ret, ⌜ret = Vundef↑⌝ ∗ stack_content γs (v :: l)))%I))).
+  Definition push_spec : fspec :=
+    fspec_winv (↑N)
+      (fspec_simple (λ '((s, v, l, γs) : val * val * list (leibnizO val) * gname),
+        ((λ arg, ⌜arg = [s; v]↑⌝ ∗ is_stack γs s 0 ∗ stack_content γs l),
+         (λ ret, ⌜ret = Vundef↑⌝ ∗ stack_content γs (v :: l)))%I)).
 End definitions.
 
 Module StackM. Section StackM.
@@ -95,9 +192,9 @@ Module StackM. Section StackM.
     λ v, ret <- lat_img false (push_spec N) 𝒴 (Ret ()) v;; 𝒴;;; Ret ret. *)
 
   Definition new_stack : Any.t → itree crisE Any.t :=
-    λ arg, ret <- lat_img false (new_stack_spec N) 𝒴 fbody_trivial arg;; 𝒴;;; Ret ret.
+    λ arg, ret <- lat_img false (from_fspec (new_stack_spec N)) 𝒴 fbody_trivial arg;; 𝒴;;; Ret ret.
   Definition push : Any.t → itree crisE Any.t :=
-    λ arg, ret <- lat_img false (push_spec N) 𝒴 fbody_trivial arg;; 𝒴;;; Ret ret.
+    λ arg, ret <- lat_img true (from_fspec (push_spec N)) 𝒴 fbody_trivial arg;; 𝒴;;; Ret ret.
 
   Definition fnsems : fnsems_type :=
     [(Some StackHdr.new_stack, (true, wmask_all, scopes, (None, new_stack)));
@@ -114,7 +211,7 @@ Module StackM. Section StackM.
   Definition t := Seal.sealing CRIS (SMod.to_mod sp_none Mod).
 End StackM. End StackM.
 
-Module StackA. Section StackA.
+(* Module StackA. Section StackA.
   Context `{!crisG Γ Σ α β τ _S _I, !concG, !memG, !stackG} (N : namespace).
   (* Module definitions *)
   Definition scopes : list string := [].
@@ -137,4 +234,4 @@ Module StackA. Section StackA.
   Next Obligation. prove_nodup. Qed.
 
   Definition t := Seal.sealing CRIS (SMod.to_mod sp_none Mod).
-End StackA. End StackA.
+End StackA. End StackA. *)
